### Definitions
String Reversal ($w^R$):
- $\epsilon$ if $w = \epsilon$
- $x^R \bullet a$ if $w = ax$

Lemma 1: $w \cdot \epsilon = w$ for any string $w$
Lemma 2: $|w\cdot x| = |w| + |x|$ for any string $w$
Lemma 3: $(w\bullet x) \bullet y = w\bullet (x\bullet y)$

#### 1) Prove $|w|$ = $|w^R|$
Proof:
Let $w$ be an arbitrary string.
IH: Assume that for every $x$ where $|x| < |w|$, that $|x| = |x^R|
Two cases:
1. $w = \epsilon$
$|w| = |\epsilon|$ (by substitution $w = \epsilon$)
$= |\epsilon^R|$ (by def. of Reversal)
$= |w^R|$ (by substitution $w = \epsilon$)

**Question**: is it a two-way implication? If $(ax)^R \rightarrow x^R\cdot a$

2. $w = ax$
$|w| = |ax|$ (by substitution $w = ax$)
$= |a| + |x|$
$= |a| + |x^R|$
$= |x^R| + |a|$
$= |x^R\cdot a|$
$= |(ax)^R|$

$= |ax|$ (by substitution $w = ax$)
$= |a| + |x|$ (by Lemma 2)
$= |a| + |x^R|$ (by I.H.)
$= |x^R| + |a|$ (by commutative property of addition)
$= |x^Ra|$ (by Lemma 2)
$= |w^R|$ 

#### Prove $(w^R)^R = w$
Proof:
Let $w$ be any arbitrary string.
I.H.: Assume that every $x$ where $|x| < |w|$, that $(x^R)^R = x$
Lemma A: For all $w, z$, $(w\bullet z)^R = z^R \bullet w^R$
Two cases:
1. $w = \epsilon$
$(w^R)^R = (\epsilon ^R)^R$ (by substitution $w = \epsilon$)
$= (\epsilon)^R$ (by def. of String Reversal)
$= \epsilon$ (by def. of String Reversal)
$= \epsilon$ (by substitution $w = \epsilon$)

2. $w = ax$
$(w^R)^R = ((ax)^R)^R$ (by substitution $w = \epsilon$)
$= (x^R\bullet a)^R$ (by def. of Reversal)
$= a^R \bullet (x^R)^R$ (by Lemma A)
$= a^R \bullet x$ (by I.H.) 
$= a \bullet x$ (by def. of Reversal?)
$= ax$ (by def. of Concatenation)
$= w$ (by substitution $w = ax$)